---
editor: 
  markdown: 
    wrap: 72
---


Perform partial fraction decomposition on $\frac{1}{A (N - A)}$: $$
\frac{1}{A (N - A)} = \frac{1}{N} \left( \frac{1}{A} + \frac{1}{N - A} \right).
$$

Integrate both sides: $$
\int \frac{1}{N} \left( \frac{1}{A} + \frac{1}{N - A} \right) dA = \int \alpha \, dt.
$$

This yields: $$
\frac{1}{N} \left( \ln|A| - \ln|N - A| \right) = \alpha t + C,
$$ where$C$is the integration constant.

Simplify: $$
\ln\left(\frac{A}{N - A}\right) = \alpha N t + C',
$$ where $C' =  N C$.

Exponentiate to solve for$A$: $$
\frac{A}{N - A} = e^{\alpha N t + C'}.
$$

Rearranging gives: $$
A = \frac{N}{1 + e^{-C' - \alpha N t}}.
$$

Finally, rewrite $e^{-C'}$ as a constant $K$: $$
A = \frac{N}{1 + K e^{-\alpha N t}},
$$ {#eq-logistic}

where $K$ depends on the initial conditions.

This is the solution for $A(t)$, and $L(t)$ can be recovered using
$L(t) = N - A(t)$.

To find $K$ for some initial condition, set $t=0$, call $A_0 = A(t=0)$,
and solve for $K$. Note that when $t=0$, the denominator in Equation
@eq-logistic becomes $1 + K$ since $e^0 = 1$. Then we have

$$
A(0) = \frac{N}{1 + K}
$$

which we can multiply by $1 + K$ on both sides and rearrange to get

$$
K = \frac{N}{A_0}.
$$
